src/Lean/RflAttrib.lean
@@ -18,7 +18,7 @@ def validateRflAttr (declName : Name) : AttrM Unit := do
         let type ← whnf type
         -- NB: The warning wording should work both for explicit uses of `@[rfl]` as well as the implicit `:= rfl`.
         let some (_, lhs, rhs) := type.eq? |
-          throwError m!"not a `rfl`-theorem: the conculsion should be an equality, but is{inlineExpr type}"
+          throwError m!"not a `rfl`-theorem: the conclusion should be an equality, but is{inlineExpr type}"
         if !(← withOptions (smartUnfolding.set · false) <| withTransparency .all <| isDefEq lhs rhs) then
           let explanation := MessageData.ofLazyM (es := #[lhs, rhs]) do
             let (lhs, rhs) ← addPPExplicitToExposeDiff lhs rhs
